Getting DbLib integration going.

Syntax.v
@@ -1,6 +1,7 @@
 Require Import DbLib.DeBruijn.
 Require Import DbLib.Environments.
 Require Import DbLib.DblibTactics.
+Require Import PartialMap.
 
 Module Syntax.
 
@@ -13,6 +14,8 @@ Inductive loc := Loc : nat -> loc.
 Inductive term : Type :=
   (* () *)
   | TUnit
+  | TTrue
+  | TFalse
   (* let () = e1 in e2 *)
   (*
   | TLetUnit : term -> term -> term
@@ -21,7 +24,8 @@ Inductive term : Type :=
   (* let (x1, x2) = e1 in e2 *)
   | TLetPair : name -> name -> term -> term
   *)
-  | TVar : name -> term
+  (* FIXME: Would be nice to use name type, but prove_*_traverse tactics choke. *)
+  | TVar : nat -> term
   | TAbs : term -> term
   | TApp : term -> term -> term
   (*
@@ -36,13 +40,11 @@ Inductive term : Type :=
   | TNew : term -> term
   | TFree : term -> term
   | TSwap : term -> term -> term -> term
-  | TLocAbs : term -> term 
+  | TLocAbs : term -> term
   | TLocApp : term -> loc -> term
   (* let |p, x| = e1 in e2 *)
   | TLetEx : loc -> name -> term -> term -> term
   *)
-  | TTrue
-  | TFalse
 .
 
 Inductive value : term -> Type :=
@@ -68,10 +70,59 @@ Inductive ty : Type :=
   | TyBool
 .
 
+(* ---------------------- *)
 (* Substitution via DbLib *)
+(* ~~~~~~~~~~~~~~~~~~~~~~ *)
+
 Instance Var_term : Var term := {
-  var := fun i => TVar (Name i)
+  var := TVar
 }.
+
+(* Traverse the variable/value structure of a term.
+   We also need a similar function for location traversal and substituion. *)
+Fixpoint traverse_term (f : nat -> nat -> term) l t :=
+  match t with
+  | TUnit => TUnit
+  | TTrue => TTrue
+  | TFalse => TFalse
+  | TVar x =>
+      f l x
+  | TAbs e =>
+      TAbs (traverse_term f (1 + l) e)
+  | TApp e1 e2 =>
+      TApp (traverse_term f l e1) (traverse_term f l e2)
+  end.
+
+Instance Traverse_term : Traverse term term := {
+  traverse := traverse_term
+}.
+
+Instance TraverseVarInjective_term : @TraverseVarInjective term _ term _.
+Proof.
+  constructor. prove_traverse_var_injective.
+Qed.
+
+Instance TraverseFunctorial_term : @TraverseFunctorial term _ term _.
+Proof.
+  constructor. prove_traverse_functorial.
+Qed.
+
+Instance TraverseRelative_term : @TraverseRelative term term _.
+Proof.
+  constructor. prove_traverse_relative.
+Qed.
+
+Instance TraverseIdentifiesVar_term : @TraverseIdentifiesVar term _ _.
+Proof.
+  constructor. prove_traverse_identifies_var.
+Qed.
+
+Instance TraverseVarIsIdentity_term : @TraverseVarIsIdentity term _ term _.
+Proof.
+  constructor. prove_traverse_var_is_identity.
+Qed.
+
+(* END DbLib definitions *)
 
 (* Note: All terms stored in contexts are closed. *)
 Definition store : Type :=
@@ -99,10 +150,17 @@ Inductive eval_ctxt : term -> term -> Prop :=
 
 (* (sigma, e) -> (sigma', e') *)
 Inductive step : store -> term -> store -> term -> Prop :=
-  | StepAppAbs :
+  | StepAppAbs : forall s e e' v,
       value v ->
-      
-      step s () s' e'
+      subst v 0 e = e' ->
+      step s (TApp (TAbs e) v) s e'
+  | StepApp1 : forall s s' e1 e1' e2,
+      step s e1 s' e1' ->
+      step s (TApp e1 e2) s' (TApp e1' e2)
+  | StepApp2 : forall s s' v1 e2 e2',
+      value v1 ->
+      step s e2 s' e2' ->
+      step s (TApp v1 e2) s' (TApp v1 e2')
 .
 
 
